cleanup

tests/test_validate_proof.lean
@@ -1,4 +1,5 @@
 import util.tactic
+import basic.conjecture_tactics
 
 meta def should_fail
   (u v : ℕ+)
@@ -17,9 +18,61 @@ end
 
 meta def should_succeed : true := by trivial
 
+/--
+ Tests the  register_conjecture_pf tactic 
+-/
+meta def test_register_conjecture_pf : tactic unit := do { 
+  let pf_term : expr := `(trivial),
+  ts ← tactic.read, 
+  ⟨nm ,new_ts⟩ ← register_conjecture_pf pf_term ts,
+  tactic.write new_ts, 
+  env ← tactic.get_env, 
+  env.get nm *> tactic.trace "register_conjecture OK"  -- succeeds iff `nm` is inside `env` 
+  }
+
+/--
+ Tests the close_old_ts_top_goal_using_conjecture tactic
+-/
+meta def test_close_old_ts_top_goal_using_conjecture (pf_term : expr) : tactic unit  := do {
+⟨ts_old, ts_narrowed⟩ ← add_conjecture "h" "false",
+tactic.write ts_old, -- ts_old has two goals ⊢false and ⊢true
+
+⟨nm ,new_ts⟩ ← register_conjecture_pf pf_term ts_narrowed,
+final_ts ← close_old_ts_top_goal_using_conjecture ts_old nm  new_ts,
+tactic.write final_ts,
+tactic.get_goal *> tactic.trace "close_old_ts_top_goal_using_conjecture OK"  -- succeeds if new tactic state only has one goal
+}
+
+namespace dummy_ns
+/--
+  Meant to test all conjecture tactics  proves that 0 = 1 -> 0 = 2 by conjecturing that 0 = 1 -> false and then using false.elim
+-/
+  meta def test_all_conjecture_tactics: tactic unit := do {
+    ⟨ts_old, ts_narrowed⟩ ← add_conjecture "h" "0 = 1 -> false",
+
+    let pf_term : expr := `(λ h, @nat.no_confusion false 0 1 h) ,
+    ⟨nm ,new_ts⟩ ← register_conjecture_pf pf_term ts_narrowed,
+
+    final_ts ← close_old_ts_top_goal_using_conjecture ts_old nm  new_ts,
+    tactic.write final_ts,
+    pure ()
+  }
+
+  lemma dummy_lemma : (0 = 1) → (0 = 2) :=
+  begin
+    test_all_conjecture_tactics,
+    intro h',
+    exact false.elim (h h'),
+  end
+
+end dummy_ns
+
 meta def main : io unit := io.run_tactic'' $ do {
   (tactic.guard_undefined `(undefined : ℕ) <|> tactic.trace "OK"),
   (tactic.guard_sorry `(sorry : ℕ) <|> tactic.trace "OK"),
   (validate_decl `should_fail) <|> tactic.trace "OK",
   validate_decl `should_succeed *> tactic.trace "OK"
 }
+
+
+
